src/compiler/core/OCL_compiler_floor2_examp.thy
@@ -52,14 +52,14 @@ section{* Translation of AST *}
 subsection{* example *}
 
 definition "print_examp_def_st_locale_distinct = \<open>distinct_oid\<close>"
-definition "print_examp_def_st_locale_metis = M.metis (List_map T.thm [print_examp_def_st_locale_distinct, \<open>distinct_length_2_or_more\<close>])"
+definition "print_examp_def_st_locale_metis = M.metis (L.map T.thm [print_examp_def_st_locale_distinct, \<open>distinct_length_2_or_more\<close>])"
 definition "print_examp_def_st_locale_aux f_ocli l = 
  (let b = \<lambda>s. Expr_basic [s] in
   map_prod
     id
-    List_flatten
-    (List_split
-      (List_map
+    L.flatten
+    (L.split
+      (L.map
         (\<lambda> name.
            let (ocli, cpt) = f_ocli name 
              ; n = inst_name ocli
@@ -75,8 +75,8 @@ definition "print_examp_def_st_locale_make f_name f_ocli f_spec l =
  (let (oid, l_fix_assum) = print_examp_def_st_locale_aux f_ocli l
     ; ty_n = \<open>nat\<close> in
   \<lparr> HolThyLocale_name = f_name
-  , HolThyLocale_header = List_flatten
-                            [ [ ( List_map (\<lambda>x. (x, Ty_base ty_n)) oid
+  , HolThyLocale_header = L.flatten
+                            [ [ ( L.map (\<lambda>x. (x, Ty_base ty_n)) oid
                                 , Some ( print_examp_def_st_locale_distinct
                                        , Expr_app \<open>distinct\<close> [let e = Expr_list oid in
                                                                 if oid = [] then Expr_annot' e (ty_n @@ \<open> list\<close>) else e])) ]
@@ -111,18 +111,18 @@ definition "print_examp_def_st_defassoc_typecheck_gen l ocl =
            ([], RBT.empty)
        of
          ([], _) \<Rightarrow> []
-       | (l, _) \<Rightarrow> rev_map (\<lambda> (Error, n) \<Rightarrow> (Error, \<open>Extra variables on rhs: \<close> @@ n)
+       | (l, _) \<Rightarrow> L.rev_map (\<lambda> (Error, n) \<Rightarrow> (Error, \<open>Extra variables on rhs: \<close> @@ n)
                             | (Warning, n) \<Rightarrow> (Warning, \<open>Duplicate variables on rhs: \<close> @@ n)) l)
       \<open> error(s)\<close> ])"
 
 definition "print_examp_def_st_defassoc_typecheck = (\<lambda> OclDefSt _ l \<Rightarrow> \<lambda> ocl.
-  (\<lambda>l_res. (List_map O'.ML l_res, ocl \<lparr> D_output_header_force := True \<rparr>))
+  (\<lambda>l_res. (L.map O'.ML l_res, ocl \<lparr> D_output_header_force := True \<rparr>))
   (print_examp_def_st_defassoc_typecheck_gen
     l
     ocl))"
 
 definition "print_examp_def_st_mapsto_gen f ocl =
-  List_map
+  L.map
     (\<lambda>(cpt, ocore).
         let b = \<lambda>s. Expr_basic [s]
           ; (ocli, exp) = case ocore of
@@ -138,20 +138,20 @@ definition "print_examp_def_st_mapsto ocl l = list_bind id id
     l)"
 
 definition "print_examp_def_st2 = (\<lambda> OclDefSt name l \<Rightarrow> \<lambda>ocl.
- (\<lambda>(l, l_st). (List_map O'.definition l, ocl \<lparr> D_input_state := (String_to_String\<^sub>b\<^sub>a\<^sub>s\<^sub>e name, l_st) # D_input_state ocl \<rparr>))
+ (\<lambda>(l, l_st). (L.map O'.definition l, ocl \<lparr> D_input_state := (String_to_String\<^sub>b\<^sub>a\<^sub>s\<^sub>e name, l_st) # D_input_state ocl \<rparr>))
   (let b = \<lambda>s. Expr_basic [s]
-     ; l = List_map (\<lambda> OclDefCoreBinding name \<Rightarrow> map_option (Pair name) (List.assoc name (D_input_instance ocl))) l
+     ; l = L.map (\<lambda> OclDefCoreBinding name \<Rightarrow> map_option (Pair name) (List.assoc name (D_input_instance ocl))) l
      ; (rbt, (map_self, map_username)) =
          (init_map_class 
            (ocl \<lparr> D_ocl_oid_start := oidReinitInh (D_ocl_oid_start ocl) \<rparr>)
-           (List_map (\<lambda> Some (_, ocli, _) \<Rightarrow> ocli | None \<Rightarrow> ocl_instance_single_empty) l)
+           (L.map (\<lambda> Some (_, ocli, _) \<Rightarrow> ocli | None \<Rightarrow> ocl_instance_single_empty) l)
           :: (_ \<Rightarrow> _ \<times> _ \<times> (_ \<Rightarrow> ((_ \<Rightarrow> nat \<Rightarrow> _ \<Rightarrow> _) \<Rightarrow> _
                         \<Rightarrow> (ocl_ty_class option \<times> (ocl_ty \<times> ocl_data_shallow) option) list) option)) \<times> _ \<times> _)
-     ; (l_st, l_assoc) = fold_list (\<lambda> o_n l_assoc.
+     ; (l_st, l_assoc) = L.mapM (\<lambda> o_n l_assoc.
            case o_n of
               Some (name, ocli, cpt) \<Rightarrow> ([(cpt, OclDefCoreBinding (name, ocli))], (ocli, cpt) # l_assoc)
             | None \<Rightarrow> ([], l_assoc)) l []
-     ; l_st = List_unique oidGetInh (List_flatten l_st) in
+     ; l_st = List_unique oidGetInh (L.flatten l_st) in
 
    ( [ Definition (Expr_rewrite (b name) \<open>=\<close> (Expr_app \<open>state.make\<close>
         ( Expr_app \<open>Map.empty\<close> (case print_examp_def_st_mapsto ocl l_st of None \<Rightarrow> [] | Some l \<Rightarrow> l)
@@ -160,26 +160,26 @@ definition "print_examp_def_st2 = (\<lambda> OclDefSt name l \<Rightarrow> \<lam
 
 definition "print_examp_def_st_dom_name name = flatten [\<open>dom_\<close>, name]"
 definition "print_examp_def_st_dom = (\<lambda> _ ocl.
- (\<lambda> l. (List_map O'.lemma l, ocl))
+ (\<lambda> l. (L.map O'.lemma l, ocl))
   (let (name, l_st) = map_prod String\<^sub>b\<^sub>a\<^sub>s\<^sub>e_to_String id (hd (D_input_state ocl))
      ; a = \<lambda>f x. Expr_app f [x]
      ; b = \<lambda>s. Expr_basic [s]
      ; d = hol_definition in
    [ Lemma
        (print_examp_def_st_dom_name name)
-       [Expr_rewrite (a \<open>dom\<close> (a \<open>heap\<close> (b name))) \<open>=\<close> (Expr_set (List_map (\<lambda>(cpt, _). Expr_oid var_oid_uniq (oidGetInh cpt)) l_st))]
+       [Expr_rewrite (a \<open>dom\<close> (a \<open>heap\<close> (b name))) \<open>=\<close> (Expr_set (L.map (\<lambda>(cpt, _). Expr_oid var_oid_uniq (oidGetInh cpt)) l_st))]
        []
        (C.by [M.auto_simp_add [d name]])]))"
 
 definition "print_examp_def_st_dom_lemmas = (\<lambda> _ ocl.
- (\<lambda> l. (List_map O'.lemmas l, ocl))
+ (\<lambda> l. (L.map O'.lemmas l, ocl))
   (let (name, _) = hd (D_input_state ocl) in
    [ Lemmas_simp \<open>\<close>
        [T.thm (print_examp_def_st_dom_name (String\<^sub>b\<^sub>a\<^sub>s\<^sub>e_to_String name))] ]))"
 
 definition "print_examp_def_st_perm_name name = flatten [\<open>perm_\<close>, name]"
 definition "print_examp_def_st_perm = (\<lambda> _ ocl.
- (\<lambda> l. (List_map O'.lemma l, ocl))
+ (\<lambda> l. (L.map O'.lemma l, ocl))
   (let (name, l_st) = map_prod String\<^sub>b\<^sub>a\<^sub>s\<^sub>e_to_String id (hd (D_input_state ocl))
      ; expr_app = let ocl = ocl \<lparr> D_ocl_oid_start := oidReinitInh (D_ocl_oid_start ocl) \<rparr> in
                   print_examp_def_st_mapsto
@@ -192,7 +192,7 @@ definition "print_examp_def_st_perm = (\<lambda> _ ocl.
          | [_] \<Rightarrow> ([], C.by [M.simp_add [d name]])
          | _ \<Rightarrow>
            ( [ M.simp_add [d name]]
-             # List_flatten (List_map (\<lambda>i_max. List_map (\<lambda>i. [M.subst_l (List_map nat_of_str [i_max - i]) (T.thm \<open>fun_upd_twist\<close>), print_examp_def_st_locale_metis]) (List.upt 0 i_max)) (List.upt 1 (List.length l_st)))
+             # L.flatten (L.map (\<lambda>i_max. L.map (\<lambda>i. [M.subst_l (L.map nat_of_str [i_max - i]) (T.thm \<open>fun_upd_twist\<close>), print_examp_def_st_locale_metis]) (List.upt 0 i_max)) (List.upt 1 (List.length l_st)))
            , C.by [M.simp]) in
    case expr_app of None \<Rightarrow> [] | Some expr_app \<Rightarrow>
    [ Lemma
@@ -203,7 +203,7 @@ definition "print_examp_def_st_perm = (\<lambda> _ ocl.
        l_last ]))"
 
 definition "print_examp_def_st_allinst = (\<lambda> _ ocl.
- (\<lambda> l. (List_map O'.lemma l, ocl))
+ (\<lambda> l. (L.map O'.lemma l, ocl))
   (let a = \<lambda>f x. Expr_app f [x]
      ; b = \<lambda>s. Expr_basic [s]
      ; d = hol_definition
@@ -220,7 +220,7 @@ definition "print_examp_def_st_allinst = (\<lambda> _ ocl.
    map_class_gen_h'_inh (\<lambda> isub_name name compare.
      let in_name = \<lambda>ocli. b (print_examp_instance_name (\<lambda>s. s @@ isub_of_str (inst_ty ocli)) (inst_name ocli))
        ; in_pers = \<lambda>ocli. a name (a (datatype_in @@ isub_of_str (inst_ty ocli)) (in_name ocli))
-       ; expr_app = List_map (\<lambda>(ocore, ocli, exp).
+       ; expr_app = L.map (\<lambda>(ocore, ocli, exp).
               ( (ocore, ocli)
               , let asty = \<lambda>e. Expr_postunary e (b (dot_astype name))
                   ; exp_annot = [( [flatten [const_oclastype, isub_of_str name, \<open>_\<close>, inst_ty ocli]]
@@ -239,11 +239,11 @@ definition "print_examp_def_st_allinst = (\<lambda> _ ocl.
                            if String_equal name name2 then exp_annot
                            else [] | _ \<Rightarrow> [])
                 | UN' \<Rightarrow> [])) expr_app
-       ; (l_asty, ((l_spec, l_spec'), l_body)) = map_prod (M.simp_add_del [] o List_flatten)
-                                                          (map_prod List_split id o List_split)
-                                                          (List_split (List_flatten (List_map snd expr_app)))
+       ; (l_asty, ((l_spec, l_spec'), l_body)) = map_prod (M.simp_add_del [] o L.flatten)
+                                                          (map_prod L.split id o L.split)
+                                                          (L.split (L.flatten (L.map snd expr_app)))
        ; only_assms = Cons (M.simp_all_only' [ T.thms \<open>assms\<close> ])
-       ; l_assum = List_flatten [ List_map (\<lambda> ((_, ocli), l).
+       ; l_assum = L.flatten [ L.map (\<lambda> ((_, ocli), l).
                                               (\<open>\<close>, True, Expr_rewrite (in_pers ocli) (if l = [] then \<open>=\<close> else \<open>\<noteq>\<close>) (b \<open>None\<close>)))
                                            expr_app
                                 , List.map_filter (map_option (\<lambda> e \<Rightarrow> (\<open>\<close>, True, e))) l_spec'] in
@@ -256,15 +256,15 @@ definition "print_examp_def_st_allinst = (\<lambda> _ ocl.
             (Expr_binop (f_expr [b name]) \<open>\<doteq>\<close> (Expr_oclset l_spec)))
        (\<lambda>lem_tit lem_assum lem_spec var_pre_post var_mk _. Lemma_assumes
          lem_tit
-         (List_flatten [ lem_assum
+         (L.flatten [ lem_assum
                        , [(\<open>\<close>, True, Expr_And \<open>a\<close> (\<lambda>var_a. Expr_rewrite (a var_pre_post (a var_mk (b var_a))) \<open>=\<close> (b var_a)))]])
          lem_spec
-         (List_map C.apply
-           (List_flatten
+         (L.map C.apply
+           (L.flatten
             [ [[M.subst (T.thm (print_examp_def_st_perm_name name_st))]]
-            , [[M.simp_only (List_map (T.thm o d)
-                                        (\<open>state.make\<close> # List_map (\<lambda>(_, OclDefCoreBinding (n, _)) \<Rightarrow> n) l_body))]]
-            , fst (fold_list (\<lambda> expr l_spec.
+            , [[M.simp_only (L.map (T.thm o d)
+                                        (\<open>state.make\<close> # L.map (\<lambda>(_, OclDefCoreBinding (n, _)) \<Rightarrow> n) l_body))]]
+            , fst (L.mapM (\<lambda> expr l_spec.
                 let mk_StrictRefEq_including = \<lambda>l.  M.rule (T.thm \<open>const_StrictRefEq\<^sub>S\<^sub>e\<^sub>t_including\<close>)
                                                   # l_asty
                                                   # l_asty
@@ -284,7 +284,7 @@ definition "print_examp_def_st_allinst = (\<lambda> _ ocl.
                         , tl l_spec
                         , ( M.blast None
                           # f (let\<^sub>O\<^sub>C\<^sub>a\<^sub>m\<^sub>l f = \<lambda>l.  M.option [M.simp_only [T.symmetric (T.thms \<open>assms\<close>)]]
-                                              # M.simp_add (List_map d [\<open>valid\<close>, \<open>OclValid\<close>, \<open>bot_fun\<close>, \<open>bot_option\<close>])
+                                              # M.simp_add (L.map d [\<open>valid\<close>, \<open>OclValid\<close>, \<open>bot_fun\<close>, \<open>bot_option\<close>])
                                               # l in
                                mk_StrictRefEq_including (M.rule (T.thm \<open>OclIncluding_cong\<close>) # f (f []))))) in
                 ( M.subst (T.thm state_update_vs_allInstances_generic)
@@ -302,7 +302,7 @@ definition "print_examp_def_st_allinst = (\<lambda> _ ocl.
 
 definition "merge_unique_gen f l = List.fold (List.fold (\<lambda>x. case f x of Some (x, v) \<Rightarrow> RBT.insert x v | None \<Rightarrow> id)) l RBT.empty"
 definition "merge_unique f l = RBT.entries (merge_unique_gen f l)"
-definition "merge_unique' = List_map snd o merge_unique (\<lambda> (a, b). ((\<lambda>x. Some (x, (a, b))) o oidGetInh) a)"
+definition "merge_unique' = L.map snd o merge_unique (\<lambda> (a, b). ((\<lambda>x. Some (x, (a, b))) o oidGetInh) a)"
 
 definition "get_state f = (\<lambda> OclDefPP _ s_pre s_post \<Rightarrow> \<lambda> ocl. 
   let get_state = let l_st = D_input_state ocl in \<lambda>OclDefPPCoreBinding s \<Rightarrow> (s, case List.assoc s l_st of None \<Rightarrow> [] | Some l \<Rightarrow> l)
@@ -318,34 +318,34 @@ definition "get_state f = (\<lambda> OclDefPP _ s_pre s_post \<Rightarrow> \<lam
 
 definition "print_pre_post_locale_aux f_ocli l =
  (let (oid, l_fix_assum) = print_examp_def_st_locale_aux f_ocli l in
-  List_flatten [oid, List_flatten (List_map (List_map fst o fst) l_fix_assum) ])"
+  L.flatten [oid, L.flatten (L.map (L.map fst o fst) l_fix_assum) ])"
 
 definition "print_pre_post_locale = get_state (\<lambda> (s_pre, l_pre) (s_post, l_post) l_pre_post. Pair
  (let f_ocli = \<lambda>(cpt, OclDefCoreBinding (_, ocli)) \<Rightarrow> (ocli, cpt) in
   print_examp_def_st_locale_make
     (\<open>pre_post_\<close> @@ s_pre @@ \<open>_\<close> @@ s_post)
     f_ocli
-    (List_map (\<lambda>(s, l). ([], Some (s, Expr_app
+    (L.map (\<lambda>(s, l). ([], Some (s, Expr_app
                                         (print_examp_def_st_locale_name s)
                                         (print_pre_post_locale_aux f_ocli l))))
               l_pre_post)
     (merge_unique' [l_pre, l_post])))"
 
 definition "print_pre_post_interp = get_state (\<lambda> _ _.
- Pair o List_map O'.interpretation o List_map
+ Pair o L.map O'.interpretation o L.map
   (\<lambda>(s, l).
     let n = print_examp_def_st_locale_name s in
     Interpretation n n (print_pre_post_locale_aux (\<lambda>(cpt, OclDefCoreBinding (_, ocli)) \<Rightarrow> (ocli, cpt)) l) (C.by [M.rule (T.thm s)])))"
 
 definition "print_pre_post_wff = get_state (\<lambda> (s_pre, l_pre) (s_post, l_post) l_pre_post ocl.
- (\<lambda> l. (List_map O'.lemma l, ocl))
+ (\<lambda> l. (L.map O'.lemma l, ocl))
   (let a = \<lambda>f x. Expr_app f [x]
      ; b = \<lambda>s. Expr_basic [s]
      ; d = hol_definition
      ; mk_n = \<lambda>s. print_examp_def_st_locale_name s @@ \<open>.\<close> @@ s in
    [ Lemma_assumes
        (flatten [\<open>basic_\<close>, s_pre, \<open>_\<close>, s_post, \<open>_wff\<close>])
-       (List_map (\<lambda> (cpt, OclDefCoreBinding (_, ocli)) \<Rightarrow>
+       (L.map (\<lambda> (cpt, OclDefCoreBinding (_, ocli)) \<Rightarrow>
                     let ty = \<lambda>s. s @@ isub_of_str (inst_ty ocli)
                       ; n = inst_name ocli in
                     (\<open>\<close>, True, Expr_rewrite 
@@ -354,7 +354,7 @@ definition "print_pre_post_wff = get_state (\<lambda> (s_pre, l_pre) (s_post, l_
                                  (Expr_oid var_oid_uniq (oidGetInh cpt))))
                  (merge_unique' [l_pre, l_post]))
        (a \<open>WFF\<close> (let\<^sub>O\<^sub>C\<^sub>a\<^sub>m\<^sub>l mk_n = b o mk_n in Expr_pair (mk_n s_pre) (mk_n s_post)))
-       (List_map snd
+       (L.map snd
          (merge_unique (\<lambda> [oid_b, oid_a] \<Rightarrow>
                           if oid_a = oid_b then
                             None
@@ -364,12 +364,12 @@ definition "print_pre_post_wff = get_state (\<lambda> (s_pre, l_pre) (s_post, l_
                                            True
                                            (Expr_rewrite (Expr_oid var_oid_uniq oid_a) \<open>\<noteq>\<close> (Expr_oid var_oid_uniq oid_b))
                                            (C.by [print_examp_def_st_locale_metis])))
-                       [List.n_lists 2 (List_map (oidGetInh o fst)
-                                                 (List_flatten (List_map snd l_pre_post)))]))
-       (C.by [M.auto_simp_add (List_map d (\<open>WFF\<close> # List_map (mk_n o fst) l_pre_post))])] ))"
+                       [List.n_lists 2 (L.map (oidGetInh o fst)
+                                                 (L.flatten (L.map snd l_pre_post)))]))
+       (C.by [M.auto_simp_add (L.map d (\<open>WFF\<close> # L.map (mk_n o fst) l_pre_post))])] ))"
 
 definition "print_pre_post_where = get_state (\<lambda> (s_pre, l_pre) (s_post, l_post) l_pre_post ocl.
- (\<lambda> l. ((List_map O'.lemma o List_flatten) l, ocl))
+ (\<lambda> l. ((L.map O'.lemma o L.flatten) l, ocl))
   (let a = \<lambda>f x. Expr_app f [x]
      ; b = \<lambda>s. Expr_basic [s]
      ; d = hol_definition
@@ -377,7 +377,7 @@ definition "print_pre_post_where = get_state (\<lambda> (s_pre, l_pre) (s_post, 
      ; f_name = \<lambda>(cpt, ocore). Some (oidGetInh cpt, ocore)
      ; rbt_pre = merge_unique_gen f_name [l_pre]
      ; rbt_post = merge_unique_gen f_name [l_post] in
-   List_map
+   L.map
      (\<lambda>x_pers_oid.
        let (x_where, l_ocore) =
            case (RBT.lookup rbt_pre x_pers_oid, RBT.lookup rbt_post x_pers_oid) of
@@ -385,7 +385,7 @@ definition "print_pre_post_where = get_state (\<lambda> (s_pre, l_pre) (s_post, 
                                                                if String_to_list s_pre = String_to_list s_post then [hd l] else l)
            | (Some ocore, None) \<Rightarrow> (\<open>OclIsDeleted\<close>, [(ocore, s_pre)])
            | (None, Some ocore) \<Rightarrow> (\<open>OclIsNew\<close>, [(ocore, s_post)]) in
-       List_map
+       L.map
          (\<lambda> (OclDefCoreBinding (name, ocli), name_st) \<Rightarrow>
            Lemma_assumes
              (flatten [var_oid_uniq, natural_of_str (case x_pers_oid of Oid i \<Rightarrow> i), s_pre, s_post, \<open>_\<close>, name_st, \<open>_\<close>, x_where])
@@ -395,7 +395,7 @@ definition "print_pre_post_where = get_state (\<lambda> (s_pre, l_pre) (s_post, 
              (Expr_binop (let\<^sub>O\<^sub>C\<^sub>a\<^sub>m\<^sub>l mk_n = b o mk_n in Expr_pair (mk_n s_pre) (mk_n s_post))
                          \<open>\<Turnstile>\<close>
                          (a x_where (b name)))
-             [C.apply [M.simp_add (List_map d (let\<^sub>O\<^sub>C\<^sub>a\<^sub>m\<^sub>l l = [ mk_n s_post, name, x_where, \<open>OclValid\<close>, const_oid_of \<open>option\<close> ] in
+             [C.apply [M.simp_add (L.map d (let\<^sub>O\<^sub>C\<^sub>a\<^sub>m\<^sub>l l = [ mk_n s_post, name, x_where, \<open>OclValid\<close>, const_oid_of \<open>option\<close> ] in
                                              case l_pre_post of [_] \<Rightarrow> l | _ \<Rightarrow> mk_n s_pre # l))]]
              (C.by [M.option [print_examp_def_st_locale_metis]]))
          l_ocore)
