src/compiler/meta/OCL_compiler_printer_Isabelle.thy
@@ -67,22 +67,22 @@ definition "s_of_dataty _ = (\<lambda> Datatype n l \<Rightarrow>
     (To_string n)
     (String_concat \<open>
                         | \<close>
-      (List_map
+      (L.map
         (\<lambda>(n,l).
          sprint2 \<open>%s %s\<close>\<acute>
            (To_string n)
-           (String_concat \<open> \<close> (List_map (\<lambda>x. sprint1 \<open>\"%s\"\<close>\<acute> (s_of_rawty x)) l))) l) ))"
+           (String_concat \<open> \<close> (L.map (\<lambda>x. sprint1 \<open>\"%s\"\<close>\<acute> (s_of_rawty x)) l))) l) ))"
 
 definition "s_of_ty_synonym _ = (\<lambda> Type_synonym n v l \<Rightarrow>
     sprint2 \<open>type_synonym %s = \"%s\"\<close>\<acute> (if v = [] then 
                                            To_string n
                                          else
-                                           s_of_rawty (Ty_apply (Ty_base n) (List_map Ty_base v)))
+                                           s_of_rawty (Ty_apply (Ty_base n) (L.map Ty_base v)))
                                         (s_of_rawty l))"
 
 fun s_of_expr where "s_of_expr e = (\<lambda>
     Expr_rewrite e1 symb e2 \<Rightarrow> sprint3 \<open>%s %s %s\<close>\<acute> (s_of_expr e1) (To_string symb) (s_of_expr e2)
-  | Expr_basic l \<Rightarrow> sprint1 \<open>%s\<close>\<acute> (String_concat \<open> \<close> (List_map To_string l))
+  | Expr_basic l \<Rightarrow> sprint1 \<open>%s\<close>\<acute> (String_concat \<open> \<close> (L.map To_string l))
   | Expr_oid tit s \<Rightarrow> sprint2 \<open>%s%d\<close>\<acute> (To_string tit) (To_oid s)
   | Expr_annot e s \<Rightarrow> sprint2 \<open>(%s::%s)\<close>\<acute> (s_of_expr e) (s_of_rawty s)
   | Expr_bind symb e1 e2 \<Rightarrow> sprint3 \<open>(%s%s. %s)\<close>\<acute> (To_string symb) (s_of_expr e1) (s_of_expr e2)
@@ -94,7 +94,7 @@ fun s_of_expr where "s_of_expr e = (\<lambda>
   | Expr_apply e l \<Rightarrow> sprint2 \<open>%s %s\<close>\<acute> (s_of_expr e) (String_concat \<open> \<close> (List.map (\<lambda> e \<Rightarrow> sprint1 \<open>%s\<close>\<acute> (s_of_expr e)) l))
   | Expr_paren p_left p_right e \<Rightarrow> sprint3 \<open>%s%s%s\<close>\<acute> (To_string p_left) (s_of_expr e) (To_string p_right)
   | Expr_if_then_else e_if e_then e_else \<Rightarrow> sprint3 \<open>if %s then %s else %s\<close>\<acute> (s_of_expr e_if) (s_of_expr e_then) (s_of_expr e_else)
-  | Expr_pure l pure \<Rightarrow> s_of_pure_term (List_map To_string l) pure) e"
+  | Expr_pure l pure \<Rightarrow> s_of_pure_term (L.map To_string l) pure) e"
 
 definition "s_of_ty_notation _ = (\<lambda> Type_notation n e \<Rightarrow>
     sprint2 \<open>type_notation %s (\"%s\")\<close>\<acute> (To_string n) (To_string e))"
@@ -125,28 +125,28 @@ definition "s_of_definition_hol _ = (\<lambda>
   where \"%s\"\<close>\<acute> (To_string name) (s_of_expr abbrev) (s_of_expr e))"
 
 definition "(s_of_ntheorem_aux_gen :: String.literal \<times> String.literal \<Rightarrow> _ \<Rightarrow> _ \<Rightarrow> _) m lacc s = 
- (let s_base = (\<lambda>s lacc. sprint2 \<open>%s[%s]\<close>\<acute> (To_string s) (String_concat \<open>, \<close> (List_map (\<lambda>(s, x). sprint2 \<open>%s %s\<close>\<acute> s x) lacc))) in
+ (let s_base = (\<lambda>s lacc. sprint2 \<open>%s[%s]\<close>\<acute> (To_string s) (String_concat \<open>, \<close> (L.map (\<lambda>(s, x). sprint2 \<open>%s %s\<close>\<acute> s x) lacc))) in
   s_base s (m # lacc))"
 
 definition "s_of_ntheorem_aux_gen_where l = 
- (\<open>where\<close>, String_concat \<open> and \<close> (List_map (\<lambda>(var, expr). sprint2 \<open>%s = \"%s\"\<close>\<acute>
+ (\<open>where\<close>, String_concat \<open> and \<close> (L.map (\<lambda>(var, expr). sprint2 \<open>%s = \"%s\"\<close>\<acute>
                                                             (To_string var)
                                                             (s_of_expr expr)) l))"
 
 definition "s_of_ntheorem_aux_gen_of l =
- (\<open>of\<close>, String_concat \<open> \<close> (List_map (\<lambda>expr. sprint1 \<open>\"%s\"\<close>\<acute> (s_of_expr expr)) l))"
+ (\<open>of\<close>, String_concat \<open> \<close> (L.map (\<lambda>expr. sprint1 \<open>\"%s\"\<close>\<acute> (s_of_expr expr)) l))"
 
 fun s_of_ntheorem_aux where "s_of_ntheorem_aux lacc e =
   ((* FIXME regroup all the 'let' declarations at the beginning *)
    (*let f_where = (\<lambda>l. (\<open>where\<close>, String_concat \<open> and \<close>
-                                        (List_map (\<lambda>(var, expr). sprint2 \<open>%s = \"%s\"\<close>\<acute>
+                                        (L.map (\<lambda>(var, expr). sprint2 \<open>%s = \"%s\"\<close>\<acute>
                                                         (To_string var)
                                                         (s_of_expr expr)) l)))
      ; f_of = (\<lambda>l. (\<open>of\<close>, String_concat \<open> \<close>
-                                  (List_map (\<lambda>expr. sprint1 \<open>\"%s\"\<close>\<acute>
+                                  (L.map (\<lambda>expr. sprint1 \<open>\"%s\"\<close>\<acute>
                                                         (s_of_expr expr)) l)))
      ; f_symmetric = (\<open>symmetric\<close>, \<open>\<close>)
-     ; s_base = (\<lambda>s lacc. sprint2 \<open>%s[%s]\<close>\<acute> (To_string s) (String_concat \<open>, \<close> (List_map (\<lambda>(s, x). sprint2 \<open>%s %s\<close>\<acute> s x) lacc))) in
+     ; s_base = (\<lambda>s lacc. sprint2 \<open>%s[%s]\<close>\<acute> (To_string s) (String_concat \<open>, \<close> (L.map (\<lambda>(s, x). sprint2 \<open>%s %s\<close>\<acute> s x) lacc))) in
    *)\<lambda> Thm_thm s \<Rightarrow> To_string s
    | Thm_thms s \<Rightarrow> To_string s
 
@@ -180,10 +180,10 @@ definition "s_of_ntheorems = (\<lambda> Thms_single thy \<Rightarrow> s_of_ntheo
                               | Thms_mult thy \<Rightarrow> s_of_ntheorem thy)"
 
 definition "s_of_ntheorem_l l = String_concat \<open>
-                            \<close> (List_map s_of_ntheorem l)"
-definition "s_of_ntheorem_l1 l = String_concat \<open> \<close> (List_map s_of_ntheorem l)"
+                            \<close> (L.map s_of_ntheorem l)"
+definition "s_of_ntheorem_l1 l = String_concat \<open> \<close> (L.map s_of_ntheorem l)"
 
-definition "s_of_ntheorems_l l = String_concat \<open> \<close> (List_map s_of_ntheorems l)"
+definition "s_of_ntheorems_l l = String_concat \<open> \<close> (L.map s_of_ntheorems l)"
 
 definition "s_of_lemmas_simp _ = (\<lambda> Lemmas_simp_thm simp s l \<Rightarrow>
     sprint3 \<open>lemmas%s%s = %s\<close>\<acute>
@@ -194,7 +194,7 @@ definition "s_of_lemmas_simp _ = (\<lambda> Lemmas_simp_thm simp s l \<Rightarro
     sprint2 \<open>lemmas%s [simp,code_unfold] = %s\<close>\<acute>
       (if String_is_empty s then \<open>\<close> else sprint1 \<open> %s\<close>\<acute> (To_string s))
       (String_concat \<open>
-                            \<close> (List_map To_string l)))"
+                            \<close> (L.map To_string l)))"
 
 definition "(s_of_attrib_genA :: (hol__thm list \<Rightarrow> String.literal)
    \<Rightarrow> String.literal \<Rightarrow> hol__thm list \<Rightarrow> String.literal) f attr l = (* error reflection: to be merged *)
@@ -211,7 +211,7 @@ definition "(s_of_attrib_genB :: (string list \<Rightarrow> String.literal)
     sprint2 \<open> %s: %s\<close>\<acute> attr (f l))"
 
 definition "s_of_attrib = s_of_attrib_genA s_of_ntheorems_l"
-definition "s_of_attrib1 = s_of_attrib_genB (\<lambda>l. String_concat \<open> \<close> (List_map To_string l))"
+definition "s_of_attrib1 = s_of_attrib_genB (\<lambda>l. String_concat \<open> \<close> (L.map To_string l))"
 
 fun s_of_tactic where "s_of_tactic expr = (\<lambda>
     Method_rule o_s \<Rightarrow> sprint1 \<open>rule%s\<close>\<acute> (case o_s of None \<Rightarrow> \<open>\<close>
@@ -222,10 +222,10 @@ fun s_of_tactic where "s_of_tactic expr = (\<lambda>
   | Method_elim s \<Rightarrow> sprint1 \<open>elim %s\<close>\<acute> (s_of_ntheorem s)
   | Method_subst asm l s =>
       let s_asm = if asm then \<open>(asm) \<close> else \<open>\<close> in
-      if List_map String_to_list l = [''0''] then
+      if L.map String_to_list l = [''0''] then
         sprint2 \<open>subst %s%s\<close>\<acute> s_asm (s_of_ntheorem s)
       else
-        sprint3 \<open>subst %s(%s) %s\<close>\<acute> s_asm (String_concat \<open> \<close> (List_map To_string l)) (s_of_ntheorem s)
+        sprint3 \<open>subst %s(%s) %s\<close>\<acute> s_asm (String_concat \<open> \<close> (L.map To_string l)) (s_of_ntheorem s)
   | Method_insert l => sprint1 \<open>insert %s\<close>\<acute> (s_of_ntheorems_l l)
   | Method_plus t \<Rightarrow> sprint1 \<open>(%s)+\<close>\<acute> (String_concat \<open>, \<close> (List.map s_of_tactic t))
   | Method_option t \<Rightarrow> sprint1 \<open>(%s)?\<close>\<acute> (String_concat \<open>, \<close> (List.map s_of_tactic t))
@@ -249,23 +249,23 @@ fun s_of_tactic where "s_of_tactic expr = (\<lambda>
   | Method_auto_simp_add_split l_simp l_split \<Rightarrow> sprint2 \<open>auto%s%s\<close>\<acute>
       (s_of_attrib \<open>simp\<close> l_simp)
       (s_of_attrib1 \<open>split\<close> l_split)
-  | Method_rename_tac l \<Rightarrow> sprint1 \<open>rename_tac %s\<close>\<acute> (String_concat \<open> \<close> (List_map To_string l))
+  | Method_rename_tac l \<Rightarrow> sprint1 \<open>rename_tac %s\<close>\<acute> (String_concat \<open> \<close> (L.map To_string l))
   | Method_case_tac e \<Rightarrow> sprint1 \<open>case_tac \"%s\"\<close>\<acute> (s_of_expr e)
   | Method_blast None \<Rightarrow> sprint0 \<open>blast\<close>\<acute>
   | Method_blast (Some n) \<Rightarrow> sprint1 \<open>blast %d\<close>\<acute> (To_nat n)
   | Method_clarify \<Rightarrow> sprint0 \<open>clarify\<close>\<acute>
   | Method_metis l_opt l \<Rightarrow> sprint2 \<open>metis %s%s\<close>\<acute> (if l_opt = [] then \<open>\<close>
                                                    else
-                                                     sprint1 \<open>(%s) \<close>\<acute> (String_concat \<open>, \<close> (List_map To_string l_opt))) (s_of_ntheorem_l1 l)) expr"
+                                                     sprint1 \<open>(%s) \<close>\<acute> (String_concat \<open>, \<close> (L.map To_string l_opt))) (s_of_ntheorem_l1 l)) expr"
 
 definition "s_of_tactic_last = (\<lambda> Command_done \<Rightarrow> \<open>done\<close>
-                                | Command_by l_apply \<Rightarrow> sprint1 \<open>by(%s)\<close>\<acute> (String_concat \<open>, \<close> (List_map s_of_tactic l_apply))
+                                | Command_by l_apply \<Rightarrow> sprint1 \<open>by(%s)\<close>\<acute> (String_concat \<open>, \<close> (L.map s_of_tactic l_apply))
                                 | Command_sorry \<Rightarrow> \<open>sorry\<close>)"
 
 definition "s_of_meth_apply_end = (
   \<lambda> Command_apply_end [] \<Rightarrow> \<open>\<close>
   | Command_apply_end l_apply \<Rightarrow> sprint1 \<open>  apply_end(%s)
-\<close>\<acute> (String_concat \<open>, \<close> (List_map s_of_tactic l_apply)))"
+\<close>\<acute> (String_concat \<open>, \<close> (L.map s_of_tactic l_apply)))"
 
 definition' \<open>s_of_meth_apply = (
   let thesis = \<open>?thesis\<close>
@@ -274,7 +274,7 @@ definition' \<open>s_of_meth_apply = (
     ; scope_thesis = \<lambda>s. scope_thesis_gen s thesis in
   \<lambda> Command_apply [] \<Rightarrow> \<open>\<close>
   | Command_apply l_apply \<Rightarrow> sprint1 \<open>  apply(%s)
-\<close>\<acute> (String_concat \<open>, \<close> (List_map s_of_tactic l_apply))
+\<close>\<acute> (String_concat \<open>, \<close> (L.map s_of_tactic l_apply))
   | Command_using l \<Rightarrow> sprint1 \<open>  using %s
 \<close>\<acute> (s_of_ntheorems_l l)
   | Command_unfolding l \<Rightarrow> sprint1 \<open>  unfolding %s
@@ -283,31 +283,31 @@ definition' \<open>s_of_meth_apply = (
   | Command_have n b e e_last \<Rightarrow> scope_thesis (sprint4 \<open>have %s%s: "%s" %s\<close>\<acute> (To_string n) (if b then \<open>[simp]\<close> else \<open>\<close>) (s_of_expr e) (s_of_tactic_last e_last))
   | Command_fix_let l l_let o_show _ \<Rightarrow>
       scope_thesis_gen
-        (sprint2 \<open>fix %s%s\<close>\<acute> (String_concat \<open> \<close> (List_map To_string l))
+        (sprint2 \<open>fix %s%s\<close>\<acute> (String_concat \<open> \<close> (L.map To_string l))
                                      (String_concat
                                        (\<open>
 \<close>                                        )
-                                       (List_map
+                                       (L.map
                                          (\<lambda>(e_name, e_body).
                                            sprint2 \<open>          let %s = "%s"\<close>\<acute> (s_of_expr e_name) (s_of_expr e_body))
                                          l_let)))
         (case o_show of None \<Rightarrow> thesis
-                      | Some l_show \<Rightarrow> sprint1 \<open>"%s"\<close>\<acute> (String_concat \<open> \<Longrightarrow> \<close> (List_map s_of_expr l_show))))\<close>
+                      | Some l_show \<Rightarrow> sprint1 \<open>"%s"\<close>\<acute> (String_concat \<open> \<Longrightarrow> \<close> (L.map s_of_expr l_show))))\<close>
 
 definition "s_of_lemma_by _ =
  (\<lambda> Lemma n l_spec l_apply tactic_last \<Rightarrow>
     sprint4 \<open>lemma %s : \"%s\"
 %s%s\<close>\<acute>
       (To_string n)
-      (String_concat \<open> \<Longrightarrow> \<close> (List_map s_of_expr l_spec))
-      (String_concat \<open>\<close> (List_map (\<lambda> [] \<Rightarrow> \<open>\<close> | l_apply \<Rightarrow> sprint1 \<open>  apply(%s)
-\<close>\<acute> (String_concat \<open>, \<close> (List_map s_of_tactic l_apply))) l_apply))
+      (String_concat \<open> \<Longrightarrow> \<close> (L.map s_of_expr l_spec))
+      (String_concat \<open>\<close> (L.map (\<lambda> [] \<Rightarrow> \<open>\<close> | l_apply \<Rightarrow> sprint1 \<open>  apply(%s)
+\<close>\<acute> (String_concat \<open>, \<close> (L.map s_of_tactic l_apply))) l_apply))
       (s_of_tactic_last tactic_last)
   | Lemma_assumes n l_spec concl l_apply tactic_last \<Rightarrow>
     sprint5 \<open>lemma %s : %s
 %s%s %s\<close>\<acute>
       (To_string n)
-      (String_concat \<open>\<close> (List_map (\<lambda>(n, b, e).
+      (String_concat \<open>\<close> (L.map (\<lambda>(n, b, e).
           sprint2 \<open>
 assumes %s\"%s\"\<close>\<acute>
             (let (n, b) = if b then (sprint1 \<open>%s[simp]\<close>\<acute> (To_string n), False) else (To_string n, String_is_empty n) in
@@ -316,17 +316,17 @@ assumes %s\"%s\"\<close>\<acute>
        @@@@
        [sprint1 \<open>
 shows \"%s\"\<close>\<acute> (s_of_expr concl)]))
-      (String_concat \<open>\<close> (List_map s_of_meth_apply l_apply))
+      (String_concat \<open>\<close> (L.map s_of_meth_apply l_apply))
       (s_of_tactic_last tactic_last)
       (String_concat \<open> \<close>
-        (List_map
+        (L.map
           (\<lambda>l_apply_e.
             sprint1 \<open>%sqed\<close>\<acute>
               (if l_apply_e = [] then
                  \<open>\<close>
                else
                  sprint1 \<open>
-%s \<close>\<acute> (String_concat \<open>\<close> (List_map s_of_meth_apply_end l_apply_e))))
+%s \<close>\<acute> (String_concat \<open>\<close> (L.map s_of_meth_apply_end l_apply_e))))
           (List.map_filter
             (\<lambda> Command_let _ _ \<Rightarrow> Some [] | Command_have _ _ _ _ \<Rightarrow> Some [] | Command_fix_let _ _ _ l \<Rightarrow> Some l | _ \<Rightarrow> None)
             (rev l_apply)))))"
@@ -346,7 +346,7 @@ definition' \<open>s_of_interpretation _ = (\<lambda> Interpretation n loc_n loc
   sprint4 \<open>interpretation %s: %s%s
 %s\<close>\<acute> (To_string n)
      (To_string loc_n)
-     (String_concat \<open>\<close> (List_map (\<lambda>s. sprint1 \<open> "%s"\<close>\<acute> (s_of_expr s)) loc_param))
+     (String_concat \<open>\<close> (L.map (\<lambda>s. sprint1 \<open> "%s"\<close>\<acute> (s_of_expr s)) loc_param))
      (s_of_tactic_last tac))\<close>
 
 end
